\documentclass[11pt,a4paper]{article}
\usepackage[latin1]{inputenc}
\usepackage[spanish]{babel}
\usepackage{amsmath}
\usepackage{amsfonts}
\usepackage{amssymb}
\usepackage{graphicx}
\usepackage[left=2cm,right=2cm,top=2cm,bottom=2cm]{geometry}
\author{Javier Lopez Y Jorge Gerrero }
\title{Hoja de trabajo 1}
\begin{document}
\begin{Huge}
Hoja de trabajo \# 3
\end{Huge}
\textbf{Javier Lopez || Jorge Guerrero }
\section*{Ejercicio \#1}
$
[\sigma (\sigma (\sigma (0)))]+[\sigma (\sigma (\sigma (\sigma (0))))] \\
s(0)=1\\ 
\sigma (\sigma (\sigma (0)))+\sigma (\sigma (\sigma (1))) \\
(\sigma (\sigma (\sigma (0)))+\sigma (\sigma (\sigma(1)))) \\
(\sigma (\sigma (\sigma (\sigma (0)))]+\sigma (\sigma (1))))\\ 
(\sigma (\sigma ([\sigma (\sigma (\sigma (0)))]+\sigma (1))))\\
(\sigma (\sigma (\sigma ([\sigma (\sigma (\sigma (0)))]+1))))\\
(\sigma (\sigma (\sigma (\sigma (\sigma (\sigma (\sigma (0+1))))))))\\
(\sigma (\sigma (\sigma (\sigma (\sigma (\sigma (\sigma (1))))))))=(\sigma (\sigma (\sigma (\sigma (\sigma (\sigma (2))))))) \\
(\sigma (\sigma (\sigma (\sigma (\sigma (3))))))=\sigma (\sigma (\sigma (4)))=\sigma (\sigma (5))=\sigma(6)=7 
$
\section*{Ejercicio \#2}
$ a \ast b = $
$\left\{
	\begin{array}{ll}
		a   \mbox{ / }  b=1 \\
		0 \mbox{ / }    a=0 \mbox{ }  \vee \mbox{ }  b=0 \\
		b+((x)*b) \mbox{ / }  a = \sigma(x)
	\end{array}
\right.$
\section*{Ejercicio \#3}
$
(\sigma(\sigma(\sigma(0)))*0 = a*0 = 0 \\
(\sigma(\sigma(\sigma(0)))*(\sigma(0) = (\sigma(0)=1 = (\sigma(\sigma(\sigma(0)))*1 = (\sigma(\sigma(\sigma(0))) = (\sigma(\sigma(1)) = \sigma(2) = 3\\
(\sigma(\sigma(\sigma(0)))*(\sigma(\sigma(0)) = 3*2 = 3+3 \vee 2+2+2 = 6
$
\section*{Ejercicio \#4}
$
a+(\sigma (\sigma (0))=(\sigma (\sigma (a))\\
(\sigma (a+\sigma (0))=(\sigma (\sigma (a)) \\
(\sigma (\sigma (a+0))=(\sigma (\sigma (a)) \\
(\sigma (\sigma (a))=(\sigma (\sigma (a)) \\
\\
a*b=b*a
\sigma (a)*b=b*\sigma (a) \\
\sigma (a)+(\sigma (a)*x)=(x*\sigma (a))+\sigma (a) \\
\sigma ((a)+(\sigma (a)*x))=\sigma ((x*\sigma (a))+\sigma (a)) \\
\sigma ((a)+(\sigma (a)*x))= \sigma ((a)+(\sigma(a)*x)) \\
\sigma (a)+(\sigma (a)*x))= \sigma (a)+(\sigma (a)*x) \\
(\sigma (a)*b))=(\sigma (a)*b) \\
a+(a*b)=a+(a*b) \\
a*b=a*b \\
\\
a*(b*c)=(a*b)*c \\
\sigma (a)*(b*c)=(\sigma (a)*b)*c \\ 
\sigma (a)*(b*c)=((\sigma (a)+(\sigma (a)*x))*c) \\
\sigma (a)*(b*c)=((\sigma (a)*(b))*c) \\
\sigma (a)*(b*c)=(\sigma (a)*(b)*c) \\
\sigma (a)*(b*c)=(\sigma (a)*b*c)  \\
\sigma (a)*(b*c)=\sigma (a)*(b*c) \\
\\
(a+b)*c=(a*c)+(b*c) \\
(\sigma (x)+b)*c=(\sigma (x)*c)+(b*c) \\ 
(\sigma(x+b)*c)=(\sigma (x)*c)+(b*c) \\ 
((\sigma (x)+b)*c)=(\sigma (x)*c)+(b*c) \\
((\sigma (x)*c)+(b*c))=(\sigma (x)*c)+(b*c) \\ 
(\sigma (x)*c)*+(b*c)=(\sigma (x)*c)+(b*c) \\
\\
(\sigma (x)*c+b*c)=(\sigma (x)*c)+(b*c) \\
(\sigma (x)*c)+(b*c)=(\sigma (x)*c)+(b*c) \\
$

\end{document}
