\documentclass[11pt,a4paper]{article}
\usepackage[latin1]{inputenc}
\usepackage[spanish]{babel}
\usepackage{amsmath}
\usepackage{amsfonts}
\usepackage{amssymb}
\usepackage{graphicx}
\usepackage[left=2cm,right=2cm,top=2cm,bottom=2cm]{geometry}
\author{Javier Lopez Y Jorge Gerrero }
\title{Hoja de trabajo 1}
\begin{document}
\begin{Huge}
Hoja de trabajo \# 4
\end{Huge}
\textbf{Javier Lopez || Jorge Guerrero }
\section*{Ejercicio \#1}
Las definiciones 1 y 4 $\in 2^{n}$
\section*{Ejercicio \#2}
$
1)\lambda x \in X.x = {(x,x*5) | x\in X} /x>0 \\
{x \in X. y \in N | \exists x = y*5} \\
2)\lambda x \in X.x = {(x,x*5) | x \in X} /x>0 \bigcap {(x,x*4) | x \in X} /x>0 \\
3)\lambda x \in X.x = {(x,x/x,x/1) | x\in X. x X n} /n={1,x} \\
4)\lambda x \in X.x = {(x,x*15) | x\in X} /x>0 \\
5)\lambda x \in X.x = {(x,x\subseteq n) | x\in X. X=42} /n= N X N X... X N_{42}\\
(x \in X. n \in N | \exists x = 42 = \sum N_{y} )/0\leq N \leq 42 \wedge y\geq 0
$
\section*{Ejercicio \#3}
$
\lambda x \in X.x = ((y,z,x) | x\in X. X\subseteq N_(50) \times N_(50) \times \\ N_{50} ) /i=4 \wedge n \leq 50 \\
(x \in X. a \wedge b \in N | \exists x = y*z \wedge i=4/y \textdiscount a=0 \\ \wedge z\textdiscount b =0/i=2 \wedge y \neq z  \wedge n \leq 50)
$
\section*{Ejercicio \#4}
$
1)\lambda x \in X.x = ((x,y) | x\in X)\\
(x \in X. y \in N | \exists y = x+x )\\
2) N -> B \\
DivisibleEntre5 (n)(1| n \textdiscount 5 = 0 \\
( 0 | n \textdiscount 5 \neq 0 \\
( not(DivisibleEntre5 (n)) | n \textdiscount 5 > 0 \\
3) f(x) \wedge g(x) \in R^(+) \\
4) (x \in X. y \in R^(+) \wedge z \in R^(+) | \exists y = g(z)) \wedge z= f(x) ) \\
$
\section*{Ejercicio \#5}
$
1) surjectiva \\
2) injectiva / x \neq 1+(1*n) | n \in N \\
3) biyectiva \\
4) biyectiva
$
\section*{Ejercicio \#6}
$
1)\lambda x \in X.x = {(x_{1},x_{2}) | X = N \times N} /x>0 \\
2) \lambda x \in X.x = {(x,z) | x\in X} /x>0 \\
{x \in X. y\in N. z \in N | \exists z = 1+(y*2)/z>1 \wedge y \geq 0} \\
3)\lambda x \in X \wedge y \in Y.x = {(x,y) | X \in N \wedge Y \in Z} \\
4)\lambda x \in B.x = (((x_(1),y_(1))(x_(2),y_(2))(x_(3),y_(3))) | \exists B_(1) \\ \times B_(2) / (0,0))) /B = {(0,0),(1,1),(0,1),(1,0)}
$
\end{document}
